

A

# Chapter 6.3 补充

## ① Example 4.

书上公式子  $e^{At} = e^{It} e^{(A-I)t}$

可是我不该说 in general

BUT!  $e^{A+B} \neq e^A e^B$ .

If  $AB=BA$

$$e^A e^B = e^B e^A = e^{A+B}$$

Proof:

- We want to show that

$$e^A e^B = e^{A+B} = e^{BA} \text{ if } AB=BA.$$

- take derivative:

$$\frac{d}{dt} (e^{t(A+B)} e^{-tA} e^{-tB})$$

$$= (A+B) e^{t(A+B)} e^{-tA} e^{-tB}$$

$$- e^{t(A+B)} A e^{-tA} e^{-tB}$$

$$- e^{t(A+B)} e^{-tA} B e^{-tB}$$

$$= (A+B-A-B) e^{t(A+B)} e^{-tA} e^{-tB} = 0$$

Since Identity matrix commutes with every matrix, the equation at the beginning is always valid.

If  $AB=BA$ .

$$e^{t(A+B)} A = A e^{t(A+B)}?$$

① 首先

If  $AB=BA$ .

$$\text{then } (A+B)^n A = A (A+B)^n$$

②

$$e^{t(A+B)} A$$

$$= \sum_{k=0}^{\infty} \frac{1}{k!} (A+B)^k A$$

$$= \sum_{k=0}^{\infty} \left[ A \frac{1}{k!} (A+B)^k \right]$$

$$= A e^{t(A+B)}$$

$\Rightarrow e^{t(A+B)}$  and  $A$  also commute.

B

但是 对于  $2 \times 2$   $A$ . 我们很容易证明 that if  $\lambda_1 = \lambda_2 = \lambda$ .

$$\text{then } (A - \lambda I)^2 = \begin{bmatrix} 0 & 0 \\ 0 & 0 \end{bmatrix}.$$

$$\text{比如 } A = \begin{bmatrix} a & b \\ c & d \end{bmatrix}$$

$$\frac{1}{2} \lambda I - \frac{1}{2} \lambda I!$$

Thus we can actually write out a simplified general formula for the case where we have shared lambda's

C

$$e^{\lambda t} = \begin{bmatrix} e^{\lambda t} & & \\ & \ddots & \\ & & e^{\lambda t} \end{bmatrix}$$

It does not look true is what I meant

OK. this looks too simple. But before you attempt to show that it is not the case.

+ think about quality.

Is left side a matrix? Yes!

OK. Now you proceed.

$$e^{\lambda t} = I + \lambda t + \frac{1}{2} (\lambda t)^2 + \frac{1}{6} (\lambda t)^3 + \dots$$

• You should see that they are all diagonal matrices.

• for each entry on the diagonal.

$$a_{ii} = 1 + \lambda_i t + \frac{1}{2} (\lambda_i t)^2 + \frac{1}{6} (\lambda_i t)^3 + \dots = e^{\lambda_i t}$$

#